Proved inlining

erasure/theories/EConstantValues.v
@@ -11,7 +11,16 @@ From MetaRocq.Erasure Require Import EPrimitive EAst EEnvMap EInduction EGlobalE
 Import Kernames.
 Import MonadNotation.
 
-
+(** We transform a program by transforming each constant into a value by thunking them, and forcing their evaluation when needed *)
+(* 
+  Values:
+  - Lambdas
+  - Constructor with values
+  - Cofixpoints
+  - Primitives (with arrays composed of values)
+  - Lazy
+  - Box 
+*)
 Fixpoint consts_to_values (t : term) : term :=
   match t with
   | tVar na => tVar na
@@ -21,7 +30,6 @@ Fixpoint consts_to_values (t : term) : term :=
   | tApp fn arg => 
       tApp (consts_to_values fn) (consts_to_values arg)
   | tConst nm => tForce (tConst nm) 
-    (* For now we apply lazy on all constants, wether they already are a value or not *)
   | tConstruct i m args => tConstruct i m (map consts_to_values args)
   | tCase i mch brs =>
       tCase i (consts_to_values mch) (map (on_snd consts_to_values) brs)
@@ -40,7 +48,7 @@ Fixpoint consts_to_values (t : term) : term :=
 .
 
 Definition consts_to_values_constant_decl (cb : constant_body) : constant_body := 
-  {| cst_body := option_map tLazy (option_map consts_to_values cb.(cst_body))|}.
+  {| cst_body := option_map (tLazy ∘ consts_to_values) cb.(cst_body)|}.
 
 
 Definition consts_to_values_global_decl (d : global_decl) : global_decl :=
@@ -51,8 +59,10 @@ Definition consts_to_values_global_decl (d : global_decl) : global_decl :=
   end.
 Definition consts_to_values_decl (d : kername * global_decl) : kername * global_decl := on_snd consts_to_values_global_decl d.
 
+
 Definition consts_to_values_env Σ : global_context := 
   List.map consts_to_values_decl Σ.
+
 
 Definition consts_to_values_program (p : program) : program :=
   (consts_to_values_env p.1, consts_to_values p.2).
@@ -63,83 +73,49 @@ From MetaRocq.Erasure Require Import EProgram EWellformed EWcbvEval.
 From MetaRocq.Common Require Import Transform.
 
 
+(* Before proving the main theorems, we prove a bunch of commuting and invariance lemmas *)
+Create HintDb consts_to_values_rw_hints.
+Ltac simple := repeat (
+    match goal with
+    | |- All _ _ => apply Forall_All 
+    | H : All _ _ |- _ => apply All_Forall in H
+    | h : ?e = Some _ |-
+        option_map _ ?e = Some _ =>
+          rewrite h
+    end ||
+    autorewrite with consts_to_values_rw_hints in * || 
+    simpl in *
+  ).
+
+Hint Rewrite @Forall_All : consts_to_values_rw_hints.
+Hint Rewrite <-@forallb_Forall : consts_to_values_rw_hints.
+Hint Rewrite <-@forallb_Forall : consts_to_values_rw_hints.
+Hint Rewrite Forall_forall : consts_to_values_rw_hints.
+Hint Rewrite @forallb_map : consts_to_values_rw_hints.
+Hint Rewrite andb_and : consts_to_values_rw_hints.
+Hint Rewrite length_map : consts_to_values_rw_hints.
+Hint Rewrite length_map : consts_to_values_rw_hints.
+Hint Rewrite <- @map_skipn : consts_to_values_rw_hints.
+Hint Rewrite @nth_error_map : consts_to_values_rw_hints.
+Hint Rewrite <-@map_repeat : consts_to_values_rw_hints.
+Hint Rewrite andb_and : consts_to_values_rw_hints.
+Hint Rewrite repeat_length : consts_to_values_rw_hints.
+
+
+Lemma is_nil_map {A B} (f : A -> B) l :
+  is_nil (map f l) = is_nil l.
+Proof.
+  now destruct l.
+Qed.
+Hint Rewrite @is_nil_map : consts_to_values_rw_hints.
+
 
 Lemma isLambda_consts_to_values (d : def term) :
-  isLambda (dbody d) -> isLambda (dbody (map_def consts_to_values d)).
+  isLambda (consts_to_values (dbody d)) = isLambda (dbody d).
 Proof.
   by destruct d as [? [] ?].
 Qed.
-
-Ltac convert_foralls :=
-  repeat match goal with
-  | |- All _ _ => apply Forall_All 
-  | H : All _ _ |- _ => apply All_Forall in H
-  | H : context[is_true (forallb _ _)] |- _ =>
-      rewrite <-forallb_Forall in H
-  | H : context[Forall _ _] |- _ => rewrite Forall_forall in H
-  | |- context[forallb _ (map _ _)] => rewrite forallb_map
-  | |- context[is_true (forallb _ _)] =>
-      rewrite <-forallb_Forall
-  | |- context[Forall _ _] => rewrite Forall_forall
-  end.
-
-Theorem wf_consts_to_values_same_ctx 
-  (efl : EEnvFlags) (flags : WcbvFlags) 
-  (t : term) (k : nat) (ctx : global_context) :
-  has_tLazy_Force ->
-  wellformed ctx k t -> 
-  wellformed ctx k (consts_to_values t).
-Proof.
-  induction t using term_forall_list_ind in k |- *; simpl in *; try easy;
-  repeat rewrite ->andb_and in *;
-  try solve[
-    repeat match goal with
-    | |- _ -> _ => intro
-    | h : _ /\ _ |- _ => destruct h
-    | |- _ /\ _ => split
-    end; easy
-  ].
-  - intros ? [? all_wf]. split; first easy.
-    now convert_foralls.
-  - intros ? [[? ?] all_wf].
-     destruct cstr_as_blocks; repeat rewrite ->andb_and in *; simpl in *.
-    + repeat split; try easy.
-      * rewrite length_map.
-        now destruct (lookup_constructor_pars_args ctx i n) 
-        as [[]|].
-      * destruct all_wf as [? ?].
-        now convert_foralls.
-    + now destruct args.
-  - intros ? (? & (wf_brs_p & wf_t) &  wf_all);
-    rewrite length_map; repeat split; try easy.
-    now convert_foralls; simpl.
-  - intros ? [[? isLambda_all] wf_fix_m]; repeat split.
-    + assumption.
-    + convert_foralls.
-      auto using isLambda_consts_to_values. 
-    + unfold wf_fix in *.
-      rewrite ->andb_and in *.
-      destruct wf_fix_m as [? all_wf].
-      rewrite length_map; split; first easy.
-      unfold test_def in *.
-      now convert_foralls; simpl.
-  - intros ? [? wf_fix_m]; repeat split; first easy.
-    unfold wf_fix in *.
-    rewrite ->andb_and in *.
-    destruct wf_fix_m as [? all_wf].
-    rewrite length_map; split; first easy.
-    unfold test_def in *.
-    now convert_foralls; simpl.
-  - intros ? [? h].
-    split.
-    + destruct p as [? []]; unfold map_prim; simpl; easy.
-    + inversion X as [| | | ? [h1 h2]]; subst; try easy.
-      unfold test_prim, test_array_model in *; simpl in *.
-      rewrite ->andb_and in *.
-      now convert_foralls.
-Qed.
-
-Create HintDb consts_to_values_rw_hints.
+Hint Rewrite @isLambda_consts_to_values : consts_to_values_rw_hints.
 
 Lemma lookup_env_consts_to_values ctx name :
   lookup_env (consts_to_values_env ctx) name = option_map (consts_to_values_global_decl) (lookup_env ctx name).
@@ -162,132 +138,66 @@ Proof.
     | |- context[match ?p with _ => _ end] =>
         let hp := fresh "h" in
         destruct p eqn:hp
-    end; try easy
+    end; easy
   ).
 Qed.
 Hint Rewrite lookup_env_consts_to_values : consts_to_values_rw_hints.
 
 
-
 Lemma lookup_inductive_consts_to_values ctx i :
   lookup_inductive (consts_to_values_env ctx) i = lookup_inductive ctx i.
 Proof. 
-  unfold lookup_inductive, lookup_minductive; simpl.
-  rewrite lookup_env_consts_to_values.
+  unfold lookup_inductive, lookup_minductive; simple.
   destruct (lookup_env ctx (inductive_mind i)) as [[? | ibody]|]; simpl; reflexivity.
 Qed.
 Hint Rewrite lookup_inductive_consts_to_values : consts_to_values_rw_hints.
 
+
 Lemma lookup_constructor_consts_to_values ctx i n :
   lookup_constructor (consts_to_values_env ctx) i n = lookup_constructor ctx i n.
 Proof.
-  rewrite
-    /consts_to_values_decl
-    /lookup_constructor
-    lookup_inductive_consts_to_values //.
+  unfold consts_to_values_decl, lookup_constructor.
+  now simple.
 Qed.
 Hint Rewrite lookup_constructor_consts_to_values : consts_to_values_rw_hints.
+
 
 Lemma lookup_constructor_pars_args_consts_to_values ctx i n :
   lookup_constructor_pars_args (consts_to_values_env ctx) i n = lookup_constructor_pars_args ctx i n.
 Proof.
-  rewrite 
-    /lookup_constructor_pars_args
-    lookup_constructor_consts_to_values //.
+  unfold lookup_constructor_pars_args.
+  now simple.
 Qed.
 Hint Rewrite lookup_constructor_pars_args_consts_to_values : consts_to_values_rw_hints.
+
 
 Lemma wf_brs_consts_to_values ctx i n :
   wf_brs (consts_to_values_env ctx) i n = wf_brs ctx i n.
 Proof.
-  rewrite 
-    /wf_brs
-    lookup_inductive_consts_to_values //.
+  unfold wf_brs.
+  now simple.
 Qed.
 Hint Rewrite wf_brs_consts_to_values : consts_to_values_rw_hints.
+
 
 Lemma lookup_projection_consts_to_values ctx i :
   lookup_projection (consts_to_values_env ctx) i = lookup_projection ctx i.
 Proof.
-  rewrite /lookup_projection lookup_constructor_consts_to_values //.
+  unfold lookup_projection.
+  now simple.
 Qed.
 Hint Rewrite lookup_projection_consts_to_values : consts_to_values_rw_hints.
+
 
 Lemma lookup_constant_consts_to_values ctx s :
   lookup_constant (consts_to_values_env ctx) s = 
   option_map consts_to_values_constant_decl (lookup_constant ctx s).
 Proof.
-  induction ctx as [|[name [|]]? ?]; first easy; simpl.
-  - rewrite /lookup_constant /=.
-    now destruct (s == name).
-  - rewrite /lookup_constant /=.
-    now destruct (s == name).
+  unfold lookup_constant.
+  simple.
+  now destruct (lookup_env ctx s) as [[]|].
 Qed.
 Hint Rewrite lookup_constant_consts_to_values : consts_to_values_rw_hints.
-
-
-
-Theorem wf_consts_to_values_env_map_ctx 
-  (efl : EEnvFlags) (flags : WcbvFlags) 
-  (t : term) (k : nat) (ctx : global_context) :
-  has_tLazy_Force ->
-  wellformed ctx k t -> 
-  wellformed (consts_to_values_env ctx) k t.
-Proof.
-  induction t using term_forall_list_ind in k |- *; simpl in *; try easy;
-  repeat rewrite ->andb_and in *;
-  try solve[
-    repeat match goal with
-    | |- _ -> _ => intro
-    | h : _ /\ _ |- _ => destruct h
-    | |- _ /\ _ => split
-    end; easy
-  ].
-  - intros ? [? all_wf]. split; first easy.
-    now convert_foralls.
-  - intros ? [? ?]; split; first easy.
-    rewrite lookup_constant_consts_to_values.
-    now destruct (lookup_constant ctx s) as [[[|]]|].
-  - intros ? [[? ?] all_wf].
-     destruct cstr_as_blocks; repeat rewrite ->andb_and in *; simpl in *.
-    + repeat split. 
-      * assumption.
-      * now rewrite lookup_constructor_consts_to_values.
-      * now rewrite lookup_constructor_pars_args_consts_to_values.
-      * destruct all_wf as [? ?].
-        now convert_foralls.
-    + rewrite lookup_constructor_consts_to_values.
-      now destruct args.
-  - intros ? (? & (wf_brs_p & wf_t) &  wf_all); 
-    repeat split; try easy.
-    + now rewrite wf_brs_consts_to_values.
-    + now convert_foralls; simpl.
-  - rewrite lookup_projection_consts_to_values.
-    now intros ? [[? ?] wf_t]; repeat split.
-  - intros ? [[? isLambda_all] wf_fix_m]; 
-    repeat split; try assumption.
-    unfold wf_fix in *.
-    rewrite ->andb_and in *.
-    destruct wf_fix_m as [? all_wf].
-    split; first easy.
-    unfold test_def in *.
-    now convert_foralls; simpl.
-  - intros ? [? wf_fix_m]; repeat split; first easy.
-    unfold wf_fix in *.
-    rewrite ->andb_and in *.
-    destruct wf_fix_m as [? all_wf].
-    split; first easy.
-    unfold test_def in *.
-    now convert_foralls; simpl.
-  - intros ? [? h].
-    split.
-    + destruct p as [? []]; unfold map_prim; simpl; easy.
-    + destruct p as [? []]; unfold map_prim; simpl; [easy..|].
-      inversion X as [| | | ? [h1 h2]]; subst.
-      unfold test_prim, test_array_model in *; simpl in *.
-      rewrite ->andb_and in *.
-      now convert_foralls.
-Qed.
 
 
 Lemma fresh_consts_to_values name ctx :
@@ -296,37 +206,10 @@ Proof.
   unfold fresh_global.
   split; 
     [intros H%Forall_map_inv | intros H; apply Forall_map];
-    convert_foralls;
+    simple;
     now intros [? [|]]; simpl.
 Qed.
 Hint Rewrite fresh_consts_to_values : consts_to_values_rw_hints.
-
-Theorem wf_glob_consts_to_values
-  (efl : EEnvFlags) (flags : WcbvFlags) 
-  (ctx : global_context) :
-  has_tLazy_Force ->
-  wf_glob ctx ->
-  wf_glob (consts_to_values_env ctx).
-Proof.
-  induction ctx as [|[? [[[|]]|?]] ? ?];
-  inversion 2; subst; constructor; now rewrite /= ?wf_consts_to_values_env_map_ctx ?wf_consts_to_values_same_ctx ?fresh_consts_to_values.
-Qed.
-
-Theorem wf_consts_to_values
-  (efl : EEnvFlags) (flags : WcbvFlags) 
-  (input : Transform.program _ term) :
-  has_tLazy_Force ->
-  wf_eprogram efl input ->
-  wf_eprogram efl (consts_to_values_program input).
-Proof.
-  destruct input as [ctx t].
-  intros ? [wf_ctx wf_t].
-  split; simpl in *.
-  - now apply wf_glob_consts_to_values.
-  - now apply 
-      wf_consts_to_values_same_ctx,
-      wf_consts_to_values_env_map_ctx.
-Qed.
 
 
 Lemma consts_to_values_atom (wfl : WcbvFlags) ctx e :
@@ -338,6 +221,7 @@ Proof.
 Qed.
 Hint Rewrite -> consts_to_values_atom : consts_to_values_rw_hints.
 
+
 Lemma consts_to_values_mkApps (e : term) (args : list term) :
   consts_to_values (mkApps e args) = mkApps (consts_to_values e) (map consts_to_values args).
 Proof.
@@ -345,6 +229,7 @@ Proof.
   rewrite /= IH //.
 Qed.
 Hint Rewrite consts_to_values_mkApps : consts_to_values_rw_hints.
+
 
 Lemma consts_to_values_csubst e1 n e2 :
   consts_to_values (ECSubst.csubst e1 n e2) =
@@ -355,57 +240,58 @@ Proof.
   - f_equal.
     rewrite !map_map_compose.
     apply All_map_eq.
-    now convert_foralls.
+    now simple.
   - f_equal.  
     rewrite !map_map_compose.
     apply All_map_eq.
-    now convert_foralls.
+    now simple.
   - f_equal; try easy.
     rewrite !map_map_compose.
     apply All_map_eq.
-    convert_foralls.
+    simple.
     intros [names t] hIn; unfold on_snd; simpl in *.
     now rewrite (X (names, t)).
   - f_equal.
     rewrite !map_map_compose.
     apply All_map_eq.
-    convert_foralls.
+    simple.
     intros [dname body rarg] hIn; unfold map_def; simpl in *.
-    now rewrite length_map (X _ hIn).
+    now rewrite (X _ hIn).
   - f_equal.
     rewrite !map_map_compose.
     apply All_map_eq.
-    convert_foralls.
-    intros [dname body rarg] hIn; unfold map_def; simpl in *.
-    now rewrite length_map (X _ hIn).
+    simple.
+    intros [dname body rarg] hIn.
+    now rewrite /map_def (X _ hIn).
   - f_equal.
     inversion X as [| | | ? [heq eq_All]]; subst; try reflexivity.
     rewrite /map_prim /= /map_array_model /= heq.
     do 3 f_equal.
     rewrite !map_map_compose.
     apply All_map_eq.
-    now convert_foralls.
+    now simple.
 Qed.
 Hint Rewrite consts_to_values_csubst : consts_to_values_rw_hints.
+
 
 Lemma consts_to_values_substl l e :
   consts_to_values (ECSubst.substl l e) =
   ECSubst.substl (map consts_to_values l) (consts_to_values e).
 Proof.
+  unfold ECSubst.substl.
   induction l as [| ? ? IH] 
     using list_ind_rev; simpl; first reflexivity.
-  rewrite /ECSubst.substl map_app !fold_left_app.
-  fold (ECSubst.substl l e); simpl.
-  fold (ECSubst.substl (map consts_to_values l) (consts_to_values e)); simpl.
-  now rewrite consts_to_values_csubst IH.
+  rewrite map_app !fold_left_app.
+  now simple.
 Qed. 
 Hint Rewrite <- consts_to_values_substl : consts_to_values_rw_hints.
+
 
 Lemma map_fix_subst mfix :
   map consts_to_values (fix_subst mfix) = fix_subst (map (map_def consts_to_values) mfix).
 Proof.
   unfold fix_subst.
-  rewrite length_map.
+  simple.
   remember #|mfix| as n eqn:heq.
   clear heq.
   induction n as [|? IH]; first reflexivity.
@@ -413,6 +299,7 @@ Proof.
   now rewrite IH.
 Qed.
 Hint Rewrite map_fix_subst : consts_to_values_rw_hints.
+
 
 Lemma consts_to_values_cunfold_fix mfix idx :
   cunfold_fix (map (map_def consts_to_values) mfix) idx =
@@ -424,6 +311,7 @@ Proof.
   now rewrite consts_to_values_substl map_fix_subst.
 Qed.
 Hint Rewrite consts_to_values_cunfold_fix : consts_to_values_rw_hints.
+
 
 Lemma map_cofix_subst mfix :
   map consts_to_values (cofix_subst mfix) = cofix_subst (map (map_def consts_to_values) mfix).
@@ -438,6 +326,7 @@ Proof.
 Qed.
 Hint Rewrite map_cofix_subst : consts_to_values_rw_hints.
 
+
 Lemma consts_to_values_cunfold_cofix mfix idx :
   cunfold_cofix (map (map_def consts_to_values) mfix) idx =
   option_map (on_snd consts_to_values) (cunfold_cofix mfix idx).
@@ -450,15 +339,12 @@ Qed.
 Hint Rewrite consts_to_values_cunfold_cofix : consts_to_values_rw_hints.
 
 
-
-
 Lemma consts_to_values_ind_isprop_and_pars ctx ind :
   inductive_isprop_and_pars (consts_to_values_env ctx) ind =
   inductive_isprop_and_pars ctx ind.
 Proof.
-  rewrite
-    /inductive_isprop_and_pars 
-    lookup_inductive_consts_to_values //.
+  unfold inductive_isprop_and_pars.
+  now simple.
 Qed.
 Hint Rewrite consts_to_values_ind_isprop_and_pars : consts_to_values_rw_hints.
 
@@ -466,9 +352,8 @@ Lemma consts_to_values_constr_isprop_pars_decl ctx ind n :
   constructor_isprop_pars_decl (consts_to_values_env ctx) ind n =
   constructor_isprop_pars_decl ctx ind n.
 Proof.
-  rewrite
-    /constructor_isprop_pars_decl 
-    lookup_constructor_consts_to_values //.
+  unfold constructor_isprop_pars_decl.
+  now simple. 
 Qed.  
 Hint Rewrite consts_to_values_constr_isprop_pars_decl : consts_to_values_rw_hints.
 
@@ -478,16 +363,15 @@ Lemma consts_to_values_declared_constant ctx c decl :
   declared_constant ctx c decl ->
   declared_constant (consts_to_values_env ctx) c (consts_to_values_constant_decl decl).
 Proof.
-  unfold declared_constant.
-  rewrite lookup_env_consts_to_values.
+  unfold declared_constant. simple.
   destruct (lookup_env ctx c); intros [=->].
   reflexivity.
 Qed.
 
 Lemma consts_to_values_cst_body  decl :
-  cst_body (consts_to_values_constant_decl decl) = option_map (fun t => tLazy (consts_to_values t)) (cst_body decl). 
+  cst_body (consts_to_values_constant_decl decl) = option_map (tLazy ∘ consts_to_values) (cst_body decl). 
 Proof.
-  destruct decl as [[?|]]; reflexivity.
+  reflexivity.
 Qed.
 Hint Rewrite consts_to_values_cst_body : consts_to_values_rw_hints.
 
@@ -509,8 +393,7 @@ Hint Rewrite consts_to_values_isLambda : consts_to_values_rw_hints.
 
 Lemma consts_to_values_isFixApp e : EAstUtils.isFixApp (consts_to_values e) = EAstUtils.isFixApp e.
 Proof.
-  unfold EAstUtils.isFixApp.
-  rewrite consts_to_values_head.
+  unfold EAstUtils.isFixApp; simple.
   destruct (EAstUtils.head e); reflexivity.
 Qed.
 Hint Rewrite consts_to_values_isFixApp : consts_to_values_rw_hints.
@@ -531,24 +414,21 @@ Hint Rewrite consts_to_values_isBox : consts_to_values_rw_hints.
 Lemma consts_to_values_isConstructApp e :
   EAstUtils.isConstructApp (consts_to_values e) = EAstUtils.isConstructApp e.
 Proof.
-  unfold EAstUtils.isConstructApp.
-  rewrite consts_to_values_head.
+  unfold EAstUtils.isConstructApp; simple.
   destruct (EAstUtils.head e); reflexivity.
 Qed.
 Hint Rewrite consts_to_values_isConstructApp : consts_to_values_rw_hints.
 
 Lemma consts_to_values_isPrimApp e : EAstUtils.isPrimApp (consts_to_values e) = EAstUtils.isPrimApp e.
 Proof.
-  unfold EAstUtils.isPrimApp.
-  rewrite consts_to_values_head.
+  unfold EAstUtils.isPrimApp; simple.
   destruct (EAstUtils.head e); reflexivity.
 Qed.
 Hint Rewrite consts_to_values_isPrimApp : consts_to_values_rw_hints.
 
 Lemma consts_to_values_isLazyApp e : EAstUtils.isLazyApp (consts_to_values e) = EAstUtils.isLazyApp e.
 Proof.
-  unfold EAstUtils.isLazyApp.
-  rewrite consts_to_values_head.
+  unfold EAstUtils.isLazyApp; simple.
   destruct (EAstUtils.head e); reflexivity.
 Qed.
 Hint Rewrite consts_to_values_isLazyApp : consts_to_values_rw_hints.
@@ -566,6 +446,67 @@ Hint Rewrite consts_to_values_iota : consts_to_values_rw_hints.
 
 
 
+(* TODO: comment *)
+Lemma wf_consts_to_values_same_ctx 
+  (efl : EEnvFlags) (flags : WcbvFlags) 
+  (t : term) (k : nat) (ctx : global_context) :
+  has_tLazy_Force ->
+  wellformed ctx k t -> 
+  wellformed ctx k (consts_to_values t).
+Proof.
+  induction t using term_forall_list_ind in k |- *;
+  simple; unfold wf_fix, test_def, map_prim, test_prim, test_array_model in *;
+  repeat split; intros; simple; try easy.
+  - now destruct cstr_as_blocks; simple.
+  - inversion X; subst; easy.
+  - inversion X as [| | | ? [? ?]]; subst; now simple.
+Qed.
+
+
+Lemma wf_consts_to_values_env_map_ctx 
+  (efl : EEnvFlags) (flags : WcbvFlags) 
+  (t : term) (k : nat) (ctx : global_context) :
+  has_tLazy_Force ->
+  wellformed ctx k t -> 
+  wellformed (consts_to_values_env ctx) k t.
+Proof.
+  induction t using term_forall_list_ind in k |- *; simple;
+  unfold wf_fix, test_def, map_prim, test_prim, test_array_model 
+  in *; repeat split; intros; simple; try easy.
+  - now destruct (lookup_constant ctx s) as [[[|]]|].
+  - now destruct cstr_as_blocks; simple.
+  - inversion X as [| | | ? [? ?]]; subst; now simple.
+Qed.
+
+
+Lemma wf_glob_consts_to_values
+  (efl : EEnvFlags) (flags : WcbvFlags) 
+  (ctx : global_context) :
+  has_tLazy_Force ->
+  wf_glob ctx ->
+  wf_glob (consts_to_values_env ctx).
+Proof.
+  induction ctx as [|[? [[[|]]|?]] ? ?];
+  inversion 2; subst; constructor; now rewrite /= ?wf_consts_to_values_env_map_ctx ?wf_consts_to_values_same_ctx ?fresh_consts_to_values.
+Qed.
+
+Theorem wf_consts_to_values
+  (efl : EEnvFlags) (flags : WcbvFlags) 
+  (input : eprogram) :
+  has_tLazy_Force ->
+  wf_eprogram efl input ->
+  wf_eprogram efl (consts_to_values_program input).
+Proof.
+  destruct input as [ctx t].
+  intros ? [wf_ctx wf_t].
+  pose proof wf_glob_consts_to_values.
+  pose proof wf_consts_to_values_same_ctx.
+  pose proof wf_consts_to_values_env_map_ctx.
+  unfold wf_eprogram.
+  now simpl.
+Qed.
+
+(* For the proof of preservation of evaluation, the induction hypotheses will have wellformedness properties as premises. This tactic specializes the ihs and tries to prove the premises *)
 #[local] Ltac destruct_IHs :=
     repeat match goal with 
     | IH : _ -> 
@@ -573,71 +514,60 @@ Hint Rewrite consts_to_values_iota : consts_to_values_rw_hints.
         |- _ =>
         unshelve epose proof IH _; first try easy;
         clear IH
-    end;[
+    end
+    ; [
       try solve[
-        repeat match goal with
-        | h : is_true (is_nil ?l) |- _ => 
-            destruct l; last (simpl in h; easy); clear h
-        | h : _ /\ _ |- _ => destruct h
-        | h : is_true (_ && _) |- _ => apply andb_andI in h
-        | h : eval _ _ _ |- _ => 
-            apply eval_wellformed in h; [|easy..]; simpl in h
-        | h : is_true (wellformed _ _ (mkApps _ _)) |- _ =>
-            rewrite wellformed_mkApps /= in h
-        | |- is_true (wellformed _ _ (iota_red _ _ _)) => 
-            eapply wellformed_iota_red_brs
-        | |- is_true (wellformed _ _ (ECSubst.csubst _ _ _)) => 
-            eapply wellformed_csubst
-        | |- is_true (wellformed _ _ (ECSubst.substl _ _)) => 
-            eapply wellformed_substl
-        | |- context[is_true (_ && _)] => rewrite andb_and
-        | |- _ /\ _ => split; try easy
-        | h : ?P |- ?P => assumption
-        | |- is_true (wellformed _ _ (mkApps _ _)) =>
-            rewrite wellformed_mkApps /=
-        | h : cunfold_fix _ _ = Some (_, ?e) |-
-            is_true (wellformed _ _ ?e) => 
-            eapply wellformed_cunfold_fix; simpl
-        | h : cunfold_cofix _ _ = Some (_, ?e) |-
-            is_true (wellformed _ _ ?e) => 
-            eapply wellformed_cunfold_cofix; simpl
-        | h : nth_error _ _ = Some ?a |-
-              is_true (wellformed _ _ ?a) => eapply nth_error_forallb
-        | h : context[if ?c then _ else _] |- _ => 
-            destruct c eqn:?
-        end; easy
+        repeat (
+          easy || simple || 
+          lazymatch goal with
+          | h : is_true (wellformed _ _ (mkApps _ _)) |- _ =>
+              rewrite wellformed_mkApps /= in h
+          | |- is_true (wellformed _ _ (mkApps _ _)) =>
+              rewrite wellformed_mkApps /=
+          | h : _ /\ _ |- _ => destruct h
+          | h : cunfold_fix _ _ = Some (_, ?e) |-
+              is_true (wellformed _ _ ?e) => 
+              eapply wellformed_cunfold_fix; simpl
+          | h : cunfold_cofix _ _ = Some (_, ?e) |-
+              is_true (wellformed _ _ ?e) => 
+              eapply wellformed_cunfold_cofix; simpl
+          | h : nth_error _ _ = Some ?a |-
+                is_true (wellformed _ _ ?a) => eapply nth_error_forallb
+          | |- is_true (wellformed _ _ (iota_red _ _ _)) => 
+              eapply wellformed_iota_red_brs
+          | |- is_true (wellformed _ _ (ECSubst.csubst _ _ _)) => 
+              eapply wellformed_csubst
+          | |- is_true (wellformed _ _ (ECSubst.substl _ _)) => 
+              eapply wellformed_substl
+          | |- _ /\ _ => split
+          | h : context[if ?c then _ else _] |- _ => 
+              destruct c eqn:?
+          | h : is_true (is_nil ?l) |- _ => 
+              destruct l; last (simpl in h; easy); clear h
+          end ||
+          match goal with
+          | h : eval _ _ _ |- _ => 
+              apply eval_wellformed in h; [|easy..]; simpl in h
+          end 
+        )
       ]..
     |].
 
-
-Hint Rewrite length_map : consts_to_values_rw_hints.
-Hint Rewrite <- @map_skipn : consts_to_values_rw_hints.
-Hint Rewrite @nth_error_map : consts_to_values_rw_hints.
-Hint Rewrite <-@map_repeat : consts_to_values_rw_hints.
-Hint Rewrite andb_and : consts_to_values_rw_hints.
-Hint Rewrite repeat_length : consts_to_values_rw_hints.
-
+(* 
+  Most cases are handled by the following tactic 
+  It is a bit slow, destruct_IHs seems to be the bottleneck
+*)
 #[local]
-Ltac my_simpl :=
-  repeat(
-    match goal with
-    | h : ?e = Some _ |-
-        option_map _ ?e = Some _ =>
-          rewrite h
-    end ||
-    autorewrite with consts_to_values_rw_hints in *
-  ).
-
-#[local]
-Ltac crush := solve[
-    destruct_IHs; my_simpl; econstructor; try now my_simpl
+Ltac crush lem := solve[
+    simple; eapply lem; try now simple
   ].
 
-Theorem trust_consts_to_values_pres :
-  forall (efl : EEnvFlags) (wfl : WcbvFlags) (p : Transform.program _ term)
+Theorem consts_to_values_pres :
+  forall (efl : EEnvFlags) (wfl : WcbvFlags) (p : eprogram)
   (v : term),
   has_tApp -> (* Needed for eval_wellformed *)
-  has_tBox -> (*  *)
+  has_tBox -> (* Needed for wellformedness in the case eval_iota_sing *)
+  (* TODO: ajouter has_tBox \/ ~ has_iota_sing *)
   wf_eprogram efl p ->
   eval_eprogram wfl p v ->
   let ip := consts_to_values_program p in
@@ -645,42 +575,41 @@ Theorem trust_consts_to_values_pres :
 Proof.
   intros ? ? [ctx e] ? ? htBox [wf_ctx wf_e] [eval_e]; simpl in *.
   constructor; simpl.
-  induction eval_e; simpl in *.
-  - crush.
-  - crush.
-  - crush.
-  - crush.
-  - crush.
-  - subst.
-    destruct_IHs; simpl in *.
+  induction eval_e; simpl in *; subst.
+  - destruct_IHs. crush eval_box.
+  - destruct_IHs. crush eval_beta.
+  - destruct_IHs. crush eval_zeta.
+  - destruct_IHs. crush eval_iota.
+  - destruct_IHs. crush eval_iota_block.
+  - destruct_IHs; simpl in *.
     { assert (
-        forall n, forallb (wellformed ctx 0) (repeat tBox n)
+        forallb (wellformed ctx 0) (repeat tBox #|n|)
       ).
-      { move: htBox; clear. induction n; simpl; now my_simpl. }
-      apply wellformed_substl; now my_simpl. }
-    eapply eval_iota_sing; try now my_simpl.
+      { move: htBox; clear. induction n; simpl; now simple. }
+      apply wellformed_substl; now simple. }
+    eapply eval_iota_sing; try now simple.
     change tBox with (consts_to_values tBox).
-    now my_simpl.
-  - crush.
-  - crush.
-  - crush.
-  - crush.
-  - crush.
+    now simple.
+  - destruct_IHs. crush eval_fix.
+  - destruct_IHs. crush eval_fix_value.
+  - destruct_IHs. crush eval_fix'.
+  - destruct_IHs. crush eval_cofix_case.
+  - destruct_IHs. crush eval_cofix_proj.
   - destruct_IHs.
     { rewrite /lookup_constant isdecl /= in wf_e.
       apply lookup_env_wellformed in isdecl; last assumption.
       rewrite /wf_global_decl e //= in isdecl. }
-    eapply eval_force; try now my_simpl.
+    eapply eval_force; try now simple.
     econstructor.
     + now apply consts_to_values_declared_constant. 
-    + now my_simpl.
+    + now simple.
     + do 2 constructor.
-  - crush.
-  - crush.
-  - crush.
-  - crush.
-  - destruct_IHs; my_simpl.
-    eapply eval_construct_block; try now my_simpl.
+  - destruct_IHs. crush eval_proj.
+  - destruct_IHs. crush eval_proj_block.
+  - destruct_IHs. crush eval_proj_prop.
+  - destruct_IHs. crush eval_construct.
+  - destruct_IHs; simple.
+    eapply eval_construct_block; try now simple.
     destruct cstr_as_blocks; last first.
     { destruct args; last easy. 
       inversion a; subst.
@@ -690,11 +619,11 @@ Proof.
     apply All2_All2_Set, All2_map.
     apply All2_over_undep in iha.
     unshelve eapply (All2_apply_dep_arrow _ iha).
-    now convert_foralls.
-  - crush.
-  - inversion X; subst; try solve[repeat constructor]; my_simpl.
+    now simple.
+  - destruct_IHs. crush eval_app_cong.
+  - inversion X; subst; try solve[repeat constructor]; simple.
     rewrite /test_prim /= /test_array_model /= in wf_e.
-    my_simpl.
+    simple.
     destruct_IHs.
     unfold map_prim; simpl.
     do 2 constructor; last assumption.
@@ -702,7 +631,61 @@ Proof.
     apply All2_All2_Set, All2_map.
     apply All2_over_undep in X0.
     unshelve eapply (All2_apply_dep_arrow _ X0).
-    now convert_foralls.
-  - crush.
-  - crush.
+    now simple.
+  - destruct_IHs. crush eval_force.
+  - destruct_IHs. crush eval_atom.
 Qed.
+
+Import Transform.
+
+Program Definition consts_to_values_transformation (efl : EEnvFlags) (wfl : WcbvFlags) (hApp : has_tApp) (hBox : has_tBox) (hLazy : has_tLazy_Force) :
+  Transform.t _ _ EAst.term EAst.term _ _
+    (eval_eprogram wfl) (eval_eprogram wfl) :=
+  {| name := "Constants to values";
+    transform p _ := consts_to_values_program p ;
+    pre p := wf_eprogram efl p ;
+    post (p : eprogram) := wf_eprogram efl p ;
+    obseq p hp (p' : eprogram) v v' := v' = consts_to_values v |}.
+
+Next Obligation.
+  now apply wf_consts_to_values.
+Qed.
+Next Obligation.
+  eexists (consts_to_values v); split; last reflexivity.
+  now eapply consts_to_values_pres.
+Qed.
+
+Lemma consts_to_values_extends ctx ctx' :
+  extends ctx ctx' ->
+  extends (consts_to_values_env ctx) (consts_to_values_env ctx').
+Proof.
+  intros h_extends name decl heq.
+  simple.
+  apply option_map_Some in heq as [decl' [heq%h_extends ?]]; subst.
+  now rewrite heq.
+Qed.
+
+#[global]
+Lemma trust_consts_to_values_transformation_ext :
+  forall (efl : EEnvFlags) (wfl : WcbvFlags) hApp hBox hLazy,
+  TransformExt.t (consts_to_values_transformation efl wfl hApp hBox hLazy)
+    (fun p p' => extends p.1 p'.1) (fun p p' => extends p.1 p'.1).
+Proof.
+  intros efl wfl hApp hBox hLazy p p' h1 h2.
+  apply consts_to_values_extends.
+Qed.
+
+Definition extends_consts_to_values_eprogram (p q : eprogram) :=
+  extends p.1 q.1 /\ p.2 = q.2.
+
+#[global]
+Theorem trust_inline_transformation_ext' :
+  forall (efl : EEnvFlags) (wfl : WcbvFlags) hApp hBox hLazy,
+  TransformExt.t (consts_to_values_transformation efl wfl hApp hBox hLazy)
+    extends_eprogram extends_consts_to_values_eprogram.
+Proof.
+  intros efl wfl hApp hBox hLazy [ctx e] [ctx' e'] h1 h2 [h_extends heq]; simple; subst.
+  pose proof consts_to_values_extends.
+  now split; simple.
+Qed.
+
